WIP compspecs parameter in malloc_token and malloc/free specs

memmgr/spec_malloc.v
@@ -15,8 +15,6 @@ Compiling malloc.c triggers a warning from a header file:
 This is ok.
 *)
 
-(* TODO remove the following *)
-
 Instance CompSpecs : compspecs. make_compspecs prog. Defined. 
 Definition Vprog : varspecs. mk_varspecs prog. Defined. 
 
@@ -108,6 +106,20 @@ needed for splittable token.
 
 The 'retainer' (TODO term?) is needed to validate malloc_token_valid_pointer;
 a small share of the user's block.
+
+REVISION IN PROGRESS:
+
+- malloc_spec and free_spec 
+  param on cs and on type (yes, free too)
+  use malloc_token param'd on cs and type
+
+- malloc_spec' and free_spec' 
+  not param'd on anything (except implicit cs in malloc context)
+  use malloc_token' param'd on size
+
+- malloc_token' param'd on size and not on cs 
+- malloc_tok is just underlying malloc_token'
+
 *)
 
 Definition comp := VST.msl.shares.Share.comp.
@@ -124,40 +136,87 @@ Definition malloc_tok (sh: share) (n: Z) (s: Z) (p: val): mpred :=
     then emp
     else memory_block Tsh WA (offset_val (-(WA+WORD)) p)).  (* waste at start of large *)
 
-Definition malloc_token (sh: share) (t: type) (p: val): mpred := 
-   EX s:Z, malloc_tok sh (sizeof t) s p.
-
+(* for export *)
 Definition malloc_token' (sh: share) (n: Z) (p: val): mpred := 
    EX s:Z, malloc_tok sh n s p.
 
+(* for export *)
+Definition malloc_token {cs: compspecs} (sh: share) (t: type) (p: val): mpred := 
+   !! field_compatible t [] p && 
+   malloc_token' sh (sizeof t) p.
 
-Lemma malloc_token_valid_pointer_size:
-  forall sh t p, malloc_token sh t p |-- valid_pointer (offset_val (- WORD) p).
+
+Lemma malloc_token'_valid_pointer_size: 
+  forall sh n p, malloc_token sh n p |-- valid_pointer (offset_val (- WORD) p).
 Proof.
-  intros; unfold malloc_token, malloc_tok; entailer!.
+  intros; unfold malloc_token, malloc_token', malloc_tok; entailer!.
   sep_apply (data_at_valid_ptr Tsh tuint (Vint (Int.repr s)) (offset_val(-WORD) p)).
   apply top_share_nonidentity.
   entailer!.
 Qed.
 
-Lemma malloc_token_local_facts:
-  forall sh t p, malloc_token sh t p 
-  |-- !!( malloc_compatible (sizeof t) p /\ 
-          0 <= (sizeof t) <= Ptrofs.max_unsigned - (WA+WORD)).
+
+Lemma malloc_token_valid_pointer_size: 
+  forall sh t p, malloc_token sh t p |-- valid_pointer (offset_val (- WORD) p).
 Proof.
-  intros; unfold malloc_token; Intro s; unfold malloc_tok; entailer!.
+  intros; unfold malloc_token, malloc_token', malloc_tok; entailer!.
+  sep_apply (data_at_valid_ptr Tsh tuint (Vint (Int.repr s)) (offset_val(-WORD) p)).
+  apply top_share_nonidentity.
+  entailer!.
+Qed.
+
+(* for export *)
+Lemma malloc_token'_local_facts:
+  forall sh n p, malloc_token' sh n p 
+  |-- !!( malloc_compatible n p /\ 0 <= n <= Ptrofs.max_unsigned - (WA+WORD)).
+Proof.
+  intros; unfold malloc_token, malloc_token'; Intro s; unfold malloc_tok; entailer!.
+  apply (malloc_compatible_prefix n s p); try omega; try assumption.
+Qed.
+
+(* for export *)
+Lemma malloc_token_local_facts:
+  forall {cs: compspecs} sh t p, malloc_token sh t p 
+  |-- !!( malloc_compatible (sizeof t) p /\ 
+          0 <= (sizeof t) <= Ptrofs.max_unsigned - (WA+WORD) /\
+          field_compatible t [] p).
+Proof.
+  intros; unfold malloc_token, malloc_token'; Intro s; unfold malloc_tok; entailer!.
   apply (malloc_compatible_prefix (sizeof t) s p); try omega; try assumption.
 Qed.
 
-Lemma malloc_token_valid_pointer:
-  forall sh t p, malloc_token sh t p |-- valid_pointer p.
+
+(* for export *)
+Lemma malloc_token'_valid_pointer:
+  forall sh n p, malloc_token' sh n p |-- valid_pointer p.
 Proof.
-  intros.  unfold malloc_token.
+  intros.  unfold malloc_token, malloc_token'.
   entailer!.
   unfold malloc_tok.
   assert_PROP (s > 0). { 
     entailer!. bdestruct(bin2sizeZ (BINS-1) <? s). rep_omega.
-    apply Znot_lt_ge in H9. apply Z.ge_le in H9. apply H1 in H9.
+    match goal with | HA: not(bin2sizeZ _ < _) |- _ => 
+      (apply Znot_lt_ge in HA; apply Z.ge_le in HA; apply H1 in HA) end.
+    pose proof (bin2size_range (size2binZ n)). subst.
+    pose proof (size2bin_range n). rep_omega.
+  }
+  sep_apply (memory_block_valid_pointer (comp Ews) s p 0); try omega.
+  apply nonidentity_comp_Ews.
+  entailer.
+Qed.
+
+
+(* for export *)
+Lemma malloc_token_valid_pointer:
+  forall {cs: compspecs} sh t p, malloc_token sh t p |-- valid_pointer p.
+Proof.
+  intros.  unfold malloc_token, malloc_token'.
+  entailer!.
+  unfold malloc_tok.
+  assert_PROP (s > 0). { 
+    entailer!. bdestruct(bin2sizeZ (BINS-1) <? s). rep_omega.
+    match goal with | HA: not(bin2sizeZ _ < _) |- _ => 
+      (apply Znot_lt_ge in HA; apply Z.ge_le in HA; apply H2 in HA) end.
     pose proof (bin2size_range (size2binZ (sizeof t))). subst.
     pose proof (size2bin_range (sizeof t)). rep_omega.
   }
@@ -167,8 +226,11 @@ Proof.
 Qed.
 
 Hint Resolve malloc_token_valid_pointer_size : valid_pointer.
+Hint Resolve malloc_token'_valid_pointer_size : valid_pointer.
 Hint Resolve malloc_token_valid_pointer : valid_pointer.
+Hint Resolve malloc_token'_valid_pointer : valid_pointer.
 Hint Resolve malloc_token_local_facts : saturate_local.
+Hint Resolve malloc_token'_local_facts : saturate_local.
 
 (*+ free lists *)
 
@@ -782,13 +844,14 @@ Qed.
 Lemma to_malloc_token_and_block:
 forall n p q s t, n = sizeof t -> 0 <= n <= bin2sizeZ(BINS-1) -> s = bin2sizeZ(size2binZ(n)) -> 
      malloc_compatible s p -> 
-  (  data_at Tsh tuint (Vptrofs (Ptrofs.repr s)) (offset_val (- WORD) p) *
+     field_compatible t [] p ->
+  ( data_at Tsh tuint (Vptrofs (Ptrofs.repr s)) (offset_val (- WORD) p) *
      ( data_at Tsh (tptr tvoid) q p *   
      memory_block Tsh (s - WORD) (offset_val WORD p) )
 |--  malloc_token Ews t p * memory_block Ews n p).
 Proof.
-  intros n p q s t Ht Hn Hs Hmc.
-  unfold malloc_token.
+  intros n p q s t Ht Hn Hs Hmc Hfc. 
+  unfold malloc_token, malloc_token'.
   Exists s.
   unfold malloc_tok.
   if_tac.
@@ -916,10 +979,11 @@ forall t n p,
        else memory_block Tsh WA (offset_val (-(WA+WORD)) p))).
 Proof.
   intros. rewrite data_at__memory_block. normalize.
-  unfold malloc_token. rewrite <- H.
+  unfold malloc_token, malloc_token'. rewrite <- H.
   replace   (EX s : Z, malloc_tok Ews n s p) 
     with (malloc_token' Ews n p) by normalize.
-  sep_apply (from_malloc_token'_and_block n p H0).
+  entailer.
+  sep_apply (from_malloc_token'_and_block (sizeof t) p H0).
   Intro s. Exists s. entailer!.
 Qed.
 
@@ -933,7 +997,7 @@ Also free allows null, as per Posix standard.
 
 (* public interface *)
 
-Definition malloc_spec'' := 
+Definition malloc_spec' := 
    DECLARE _malloc
    WITH n:Z, gv:globals
    PRE [ _nbytes OF size_t ]
@@ -947,7 +1011,7 @@ Definition malloc_spec'' :=
              if eq_dec p nullval then emp
              else (malloc_token' Ews n p * memory_block Ews n p)).
 
-Definition malloc_spec {cs: compspecs } (t: type):= 
+Definition malloc_spec {cs: compspecs} (t: type):= 
    DECLARE _malloc
    WITH gv:globals
    PRE [ _nbytes OF size_t ]
@@ -964,9 +1028,39 @@ Definition malloc_spec {cs: compspecs } (t: type):=
              else (malloc_token Ews t p * data_at_ Ews t p)).
 
 
+Definition free_spec' :=
+ DECLARE _free
+   WITH n:Z, p:val, gv: globals
+   PRE [ _p OF tptr tvoid ]
+       PROP ()
+       LOCAL (temp _p p; gvars gv)
+       SEP (mem_mgr gv;
+              if eq_dec p nullval then emp
+              else (malloc_token' Ews n p * memory_block Ews n p))
+    POST [ Tvoid ]
+       PROP ()
+       LOCAL ()
+       SEP (mem_mgr gv).
+
+Definition free_spec {cs:compspecs} (t: type) := 
+   DECLARE _free
+   WITH p:val, gv:globals
+   PRE [ _p OF tptr tvoid ]
+       PROP ()
+       LOCAL (temp _p p; gvars gv)
+       SEP (mem_mgr gv; 
+            if eq_dec p nullval then emp
+            else (malloc_token Ews t p * data_at_ Ews t p))
+   POST [ Tvoid ]
+       PROP ()
+       LOCAL ( )
+       SEP (mem_mgr gv).
+
+
+
 Lemma malloc_spec_sub:
  forall {cs: compspecs} (t: type), 
-   funspec_sub (snd malloc_spec'') (snd (malloc_spec t)).
+   funspec_sub (snd malloc_spec') (snd (malloc_spec t)).
 Proof.
 intros.
 apply NDsubsume_subsume.
@@ -982,11 +1076,10 @@ entailer!.
 match goal with |- _ |-- prop ?PP => set (P:=PP) end.
 entailer!.
 subst P.
-Intros p.
-Exists p.
+Intros p; Exists p.
 entailer!.
 if_tac; auto.
-unfold malloc_token.
+unfold malloc_token, malloc_token'.
 assert_PROP (field_compatible t [] p).
 entailer!.
 apply malloc_compatible_field_compatible; auto.
@@ -996,33 +1089,37 @@ unfold malloc_compatible.
 destruct H as [Ht0 Ht].
 split; try (unfold natural_alignment; auto).
 admit. (* TODO lost alignment from pre *)
-- unfold malloc_token'.
-  Intros s.
-  Exists s.
+- Intros s; Exists s.
   entailer!.
   rewrite memory_block_data_at_; auto.
-  entailer!.
-  Set Printing All.
-  admit. (* TODO cs versus CompSpecs *)
 all: fail.
 Admitted.
 
 
+Lemma free_spec_sub:
+ forall {cs: compspecs} (t: type), 
+   funspec_sub (snd free_spec') (snd (free_spec t)).
+Proof.
+intros.
+apply NDsubsume_subsume.
+split; extensionality x; reflexivity.
+split3; auto.
+intros (p,gv).
+simpl in gv.
+Exists (sizeof t, p, gv) emp.
+change (liftx emp) with (@emp (environ->mpred) _ _).
+rewrite !emp_sepcon.
+apply andp_right.
+if_tac.
+entailer!.
+entailer!. simpl in H0.
+unfold malloc_token. entailer!.
+apply data_at__memory_block_cancel.
+apply prop_right.
+entailer!.
+Qed.
 
-(*Definition free_spec {cs:compspecs} := *)
-Definition free_spec := 
-   DECLARE _free
-   WITH t:_, p:_, gv:globals
-   PRE [ _p OF tptr tvoid ]
-       PROP ()
-       LOCAL (temp _p p; gvars gv)
-       SEP (mem_mgr gv; 
-            if eq_dec p nullval then emp
-            else (malloc_token Ews t p * data_at_ Ews t p))
-   POST [ Tvoid ]
-       PROP ()
-       LOCAL ( )
-       SEP (mem_mgr gv).
+
 
 (* other functions *)
 
@@ -1110,13 +1207,6 @@ Definition free_small_spec :=
        SEP (mem_mgr gv).
 
 
-
-
-Definition Gprog : funspecs := 
- ltac:(with_library prog [ 
-   mmap0_spec; munmap_spec; bin2size_spec; size2bin_spec; fill_bin_spec;
-   malloc_small_spec; malloc_large_spec; free_small_spec; malloc_spec; 
-   free_spec]).
 
 
 
